Challenge/Modexp/Submission/Proofs/Bytecode/Artifact.lean
@@ -2460,7 +2460,7 @@ def submissionInstructions : List Instr :=
  YulEvmCompiler.Instr.op (EvmSemantics.Operation.Dup { idx := 6 }),
  YulEvmCompiler.Instr.op EvmSemantics.Operation.CALLDATALOAD,
  YulEvmCompiler.Instr.push 1 1,
- YulEvmCompiler.Instr.op EvmSemantics.Operation.MOD,
+YulEvmCompiler.Instr.op EvmSemantics.Operation.LT,
  YulEvmCompiler.Instr.op EvmSemantics.Operation.MUL,
  YulEvmCompiler.Instr.push 0 0,
  YulEvmCompiler.Instr.op EvmSemantics.Operation.MSTORE,
